generalize fold language wrt. scalar types

src/lowparse/LowParse.Spec.Fold.fst
@@ -1,50 +1,72 @@
 module LowParse.Spec.Fold
+include LowParse.Spec.Combinators
 
 module U8 = FStar.UInt8
-
-noeq
-type typ =
-| TU8
-| TPair: typ -> typ -> typ
-| TList: (elt: typ) -> typ
-| TChoice: (bool -> typ) -> typ
-
-let type_of_payload
-  (f: bool -> typ { forall x . f x << TChoice f })
-  (type_of_typ: (t: typ { t << TChoice f }) -> Tot Type0)
-  (x: bool)
-: Tot Type0
-= type_of_typ (f x)
+module SZ = LowParse.Steel.StdInt
 
 // to be used with delta_attr to compute the Steel code synthesis
 // before extraction to C
 noeq type specialize : Type0 =
 
+[@@specialize]
+noeq
+type typ
+  (#scalar_t: Type)
+  (type_of_scalar: (scalar_t -> Type))
+=
+| TScalar: scalar_t -> typ type_of_scalar
+| TPair: typ type_of_scalar -> typ type_of_scalar -> typ type_of_scalar
+| TList: (s: scalar_t) -> (sz: (type_of_scalar s -> SZ.size_t) {synth_injective sz}) -> (elt: typ type_of_scalar) -> typ type_of_scalar
+| TIf: (b: bool) -> (squash (b == true) -> typ type_of_scalar) -> (squash (b == false) -> typ type_of_scalar) -> typ type_of_scalar
+| TChoice: (s: scalar_t) -> (type_of_scalar s -> typ type_of_scalar) -> typ type_of_scalar
+
+let type_of_payload
+  (#scalar_t: Type)
+  (type_of_scalar: (scalar_t -> Type))
+  (s: scalar_t)
+  (f: type_of_scalar s -> typ type_of_scalar { forall (x: type_of_scalar s) . f x << TChoice s f })
+  (type_of_typ: (t: typ type_of_scalar { t << TChoice s f }) -> Tot Type0)
+  (x: type_of_scalar s)
+: Tot Type0
+= type_of_typ (f x)
+
 [@@specialize] // mostly for scalar types
-let rec type_of_typ (t: typ) : Tot Type0 = match t with
-| TU8 -> U8.t
+let rec type_of_typ
+  (#scalar_t: Type)
+  (#type_of_scalar: (scalar_t -> Type))
+  (t: typ type_of_scalar)
+: Tot Type
+= match t with
+| TScalar s -> type_of_scalar s
 | TPair t1 t2 -> (type_of_typ t1 & type_of_typ t2)
-| TList t' -> list (type_of_typ t') // we ignore the serializer for now
-| TChoice f -> dtuple2 bool (type_of_payload f type_of_typ)
+| TList _ _ t' -> list (type_of_typ t') // we ignore the serializer for now
+| TIf b ttrue tfalse -> if b then type_of_typ (ttrue ()) else type_of_typ (tfalse ())
+| TChoice s f -> dtuple2 (type_of_scalar s) (type_of_payload type_of_scalar s f type_of_typ)
 
 let type_of_payload'
-  (f: bool -> typ)
-: Pure (bool -> Type0)
+  (#scalar_t: Type)
+  (#type_of_scalar: (scalar_t -> Type))
+  (s: scalar_t)
+  (f: type_of_scalar s -> typ type_of_scalar)
+: Pure (type_of_scalar s -> Type)
     (requires True)
     (ensures (fun v ->
-      type_of_typ (TChoice f) == dtuple2 bool v /\
+      type_of_typ (TChoice s f) == dtuple2 (type_of_scalar s) v /\
       (forall x . v x == type_of_typ (f x))
     ))
 = let v = fun x -> type_of_typ (f x) in
-  assert_norm (type_of_typ (TChoice f) == dtuple2 bool v);
+  assert_norm (type_of_typ (TChoice s f) == dtuple2 (type_of_scalar s) v);
   v
 
 let mk_choice_value
-  (tag: bool)
-  (f: bool -> typ)
+  (#scalar_t: Type)
+  (#type_of_scalar: (scalar_t -> Type))
+  (s: scalar_t)
+  (tag: type_of_scalar s)
+  (f: (type_of_scalar s -> typ type_of_scalar))
   (v: type_of_typ (f tag))
-: Tot (type_of_typ (TChoice f))
-= let v' : dtuple2 bool (type_of_payload' f) = (| tag, v |) in
+: Tot (type_of_typ (TChoice s f))
+= let v' : dtuple2 (type_of_scalar s) (type_of_payload' s f) = (| tag, v |) in
   v'
 
 let stt (#state_i: Type) (state_t: (state_i -> Type)) (ret_t: Type) (pre: state_i) (post: (state_i)) : Tot Type = (state_t pre -> Tot (ret_t & state_t (post)))
@@ -99,12 +121,13 @@ let fold_list
 let fold_choice
   #state_i #state_t
   (#ret_t: Type)
-  (#t: bool -> Type)
+  (#tk: Type)
+  (#t: tk -> Type)
   (#pre: state_i)
   (#post: _)
-  (f: (x: bool) -> fold_t state_t (t x) ret_t pre post)
-: Tot (fold_t state_t (dtuple2 bool t) ret_t pre post)
-= fun w -> if (dfst w) then f true (dsnd w) else f false (dsnd w)
+  (f: (x: tk) -> fold_t state_t (t x) ret_t pre post)
+: Tot (fold_t state_t (dtuple2 tk t) ret_t pre post)
+= fun w -> f (dfst w) (dsnd w)
 
 let bind_fold
   #state_t
@@ -212,118 +235,143 @@ let array_index_reverse = {
 
 noeq
 type prog
+  (#scalar_t: Type)
+  (type_of_scalar: (scalar_t -> Type))
   (#state_i: Type)
   (state_t: state_i -> Type)
   (action_t: (ret_t: Type) -> (pre: state_i) -> (post: state_i) -> Type)
-: (t: typ) -> (ret_t: Type) -> state_i -> (state_i) -> Type
+: (t: typ type_of_scalar) -> (ret_t: Type) -> state_i -> (state_i) -> Type
 = | PRet:
       (#ret_t: Type) ->
       (#i: state_i) ->
-      (#t: typ) ->
+      (#t: typ type_of_scalar) ->
       (v: ret_t) ->
-      prog state_t action_t t ret_t i (i)
+      prog type_of_scalar state_t action_t t ret_t i (i)
   | PAction:
-      (#t: typ) ->
+      (#t: typ type_of_scalar) ->
       (#ret_t: Type) -> (#pre: _) -> (#post: _) ->
       action_t ret_t pre post ->
-      prog state_t action_t t ret_t pre post
+      prog type_of_scalar state_t action_t t ret_t pre post
   | PBind:
-      (#t: typ) ->
+      (#t: typ type_of_scalar) ->
       (#ret1: Type) ->
       (#pre1: _) ->
       (#post1: _) ->
       (#ret2: _) ->
       (#post2: _) ->
-      (f: prog state_t action_t t ret1 pre1 post1) ->
-      (g: ((x: ret1) -> prog state_t action_t t ret2 (post1) post2)) ->
-      prog state_t action_t t ret2 pre1 post2
-  | PIf:
-      (#t: typ) ->
+      (f: prog type_of_scalar state_t action_t t ret1 pre1 post1) ->
+      (g: ((x: ret1) -> prog type_of_scalar state_t action_t t ret2 (post1) post2)) ->
+      prog type_of_scalar state_t action_t t ret2 pre1 post2
+  | PIfP:
+      (#t: typ type_of_scalar) ->
       (#ret: Type) ->
       (#pre: state_i) ->
       (#post: state_i) ->
       (x: bool) ->
-      (squash (x == true) -> prog state_t action_t t ret pre post) ->
-      (squash (x == false) -> prog state_t action_t t ret pre post) ->
-      prog state_t action_t t ret pre post
-  | PU8:
+      (squash (x == true) -> prog type_of_scalar state_t action_t t ret pre post) ->
+      (squash (x == false) -> prog type_of_scalar state_t action_t t ret pre post) ->
+      prog type_of_scalar state_t action_t t ret pre post
+  | PIfT:
+      (#ret_t: Type) ->
+      (#pre: state_i) ->
+      (#post: state_i) ->
+      (b: bool) ->
+      (#ttrue: (squash (b == true) -> typ type_of_scalar)) ->
+      (ptrue: (squash (b == true) -> prog type_of_scalar state_t action_t (ttrue ()) ret_t pre post)) ->
+      (#tfalse: (squash (b == false) -> typ type_of_scalar)) ->
+      (pfalse: (squash (b == false) -> prog type_of_scalar state_t action_t (tfalse ()) ret_t pre post)) ->
+      prog type_of_scalar state_t action_t (TIf b ttrue tfalse) ret_t pre post
+  | PScalar:
       // the base action on a leaf type just reads the value;
       // use PBind with PAction and others to perform operations on that value
       (i: state_i) ->
-      prog state_t action_t TU8 U8.t i (i)
+      (s: scalar_t) ->
+      prog type_of_scalar state_t action_t (TScalar s) (type_of_scalar s) i (i)
   | PPair:
       (#t1: _) ->
       (#t2: _) ->
       (#ret1: _) ->
       (#pre1: _) ->
       (#post1: _) ->
-      (f1: prog state_t action_t t1 ret1 pre1 post1) ->
+      (f1: prog type_of_scalar state_t action_t t1 ret1 pre1 post1) ->
       (#ret2: _) ->
       (#post2: _) ->
-      (f2: ((x: ret1) -> prog state_t action_t t2 ret2 (post1) post2)) ->
-      prog state_t action_t (TPair t1 t2) ret2 pre1 post2
+      (f2: ((x: ret1) -> prog type_of_scalar state_t action_t t2 ret2 (post1) post2)) ->
+      prog type_of_scalar state_t action_t (TPair t1 t2) ret2 pre1 post2
   | PList:
-      (#t: typ) ->
+      (#t: typ type_of_scalar) ->
+      (s: scalar_t) ->
+      (sz: (type_of_scalar s -> SZ.size_t) {synth_injective sz}) ->
       (inv: _) ->
-      prog state_t action_t t unit inv (inv) ->
-      prog state_t action_t (TList t) unit inv (inv)
+      prog type_of_scalar state_t action_t t unit inv (inv) ->
+      prog type_of_scalar state_t action_t (TList s sz t) unit inv (inv)
   | PListFor:
-      (#t: typ) ->
+      (#t: typ type_of_scalar) ->
+      (s: scalar_t) ->
+      (sz: (type_of_scalar s -> SZ.size_t) {synth_injective sz}) ->
       (inv: _) ->
       (idx: array_index_fn) ->
-      prog state_t action_t t unit inv (inv) ->
-      prog state_t action_t (TList t) unit inv (inv)
+      prog type_of_scalar state_t action_t t unit inv (inv) ->
+      prog type_of_scalar state_t action_t (TList s sz t) unit inv (inv)
   | PChoice:
-      (#t: (bool -> typ)) ->
+      (#s: scalar_t) ->
+      (#t: (type_of_scalar s -> typ type_of_scalar)) ->
       (#ret_t: Type) ->
       (#pre: _) ->
       (#post: _) ->
-      ((x: bool) -> prog state_t action_t (t x) ret_t pre post) ->
-      prog state_t action_t (TChoice t) ret_t pre post
+      ((x: type_of_scalar s) -> prog type_of_scalar state_t action_t (t x) ret_t pre post) ->
+      prog type_of_scalar state_t action_t (TChoice s t) ret_t pre post
 
 [@@specialize; noextract_to "krml"]
 let typ_of_prog
+  (#scalar_t: Type)
+  (#type_of_scalar: (scalar_t -> Type))
   (#state_i: Type)
   (#state_t: state_i -> Type)
   (#action_t: (ret_t: Type) -> (pre: state_i) -> (post: state_i) -> Type)
-  (#t: typ)
+  (#t: typ type_of_scalar)
   (#ret_t: Type)
   (#pre: state_i)
   (#post: state_i)
-  (p: prog state_t action_t t ret_t pre post)
-: Tot typ
+  (p: prog type_of_scalar state_t action_t t ret_t pre post)
+: Tot (typ type_of_scalar)
 = t
 
 let rec sem
+  (#scalar_t: Type)
+  (#type_of_scalar: (scalar_t -> Type))
   #state_t
   (#action_t: (t: Type) -> (pre: _) -> (post: _) -> Type)
   (action_sem: ((#t: Type) -> (#pre: _) -> (#post: _) -> action_t t pre post -> stt state_t t pre post))
-  (#t: typ)
+  (#t: typ type_of_scalar)
   (#ret_t: Type)
   (#pre: _)
   (#post: _)
-  (p: prog state_t action_t t ret_t pre post)
+  (p: prog type_of_scalar state_t action_t t ret_t pre post)
 : Tot (fold_t state_t (type_of_typ t) ret_t pre post)
   (decreases p)
 = match p returns (fold_t state_t (type_of_typ t) ret_t pre post) with
   | PRet v -> action_fold (ret v) <: fold_t state_t (type_of_typ t) ret_t _ (_)
   | PAction a -> action_fold (action_sem a)
   | PBind s p -> bind_fold (sem action_sem s) (fun x -> sem action_sem (p x))
-  | PIf x ptrue pfalse -> if x then sem action_sem (ptrue ()) else sem action_sem (pfalse ())
-  | PU8 _ -> fold_read () <: fold_t state_t (type_of_typ t) ret_t _ (_)
+  | PIfP x ptrue pfalse -> if x then sem action_sem (ptrue ()) else sem action_sem (pfalse ())
+  | PIfT x ptrue pfalse -> if x then coerce _ (sem action_sem (ptrue ())) else coerce _ (sem action_sem (pfalse ()))
+  | PScalar _ _ -> fold_read () <: fold_t state_t (type_of_typ t) ret_t _ (_)
   | PPair p1 p2 -> fold_pair (sem action_sem p1) (fun r -> sem action_sem (p2 r))
-  | PList inv p -> fold_list inv (sem action_sem p)
-  | PListFor inv idx p -> fold_for_list inv (sem action_sem p) idx.array_index_f_nat
-  | PChoice #_ #_ #_ #t p -> fold_choice #_ #_ #_ #(type_of_payload' t) (fun x -> sem action_sem (p x))
+  | PList _ _ inv p -> fold_list inv (sem action_sem p)
+  | PListFor _ _ inv idx p -> fold_for_list inv (sem action_sem p) idx.array_index_f_nat
+  | PChoice #_ #_ #_ #_ #_ #s #t p -> fold_choice #_ #_ #_ #_ #(type_of_payload' s t) (fun x -> sem action_sem (p x))
 
 let pseq
+  (#scalar_t: Type)
+  (#type_of_scalar: (scalar_t -> Type))
   #state_t #action_t
-  (#t: typ)
+  (#t: typ type_of_scalar)
   (#pre1: _)
   (#post1: _)
   (#ret2: _)
   (#post2: _)
-  (f: prog state_t action_t t unit pre1 post1)
-  (g: prog state_t action_t t ret2 (post1) post2)
-: Tot (prog state_t action_t t ret2 pre1 post2)
+  (f: prog type_of_scalar state_t action_t t unit pre1 post1)
+  (g: prog type_of_scalar state_t action_t t ret2 (post1) post2)
+: Tot (prog type_of_scalar state_t action_t t ret2 pre1 post2)
 = PBind f (fun _ -> g)
